txn-data-consistency/Tapir_Falsification.thy
@@ -6,6 +6,99 @@ begin
 
 subsection \<open>Lemmas and Invariants\<close>
 
+lemma cl_commit_svrs_unchanged [dest]:
+  "s' = s \<lparr>cls := (cls s) (x1 := cls s x1 \<lparr>cl_state := A, cl_view := B\<rparr>), commit_order := C\<rparr>
+    \<Longrightarrow> svrs s' = svrs s" by auto
+
+lemma occ_check_res:
+  "occ_check k t ts rto wvo s \<in> {aborted, prepared ts rto wvo}"
+  by (simp add: occ_check_def)
+
+lemma read_resp_abs_committed_reads_inv:
+  assumes "svr_state (svrs s k) (Tn t) = idle"
+  shows
+    "abs_committed_reads (s \<lparr>svrs := (svrs s)
+      (k := svrs s k \<lparr>svr_state := (svr_state (svrs s k)) (Tn t := read X)\<rparr>)\<rparr>) k' t_wr =
+     abs_committed_reads s k' t_wr"
+  using assms
+  by (auto simp add: abs_committed_reads_def read_resp_def)
+
+definition Svr_Ver_Ord_Non_Emp where
+  "Svr_Ver_Ord_Non_Emp s k \<longleftrightarrow> svr_ver_order (svrs s k) \<noteq> []"
+                                                           
+lemmas Svr_Ver_Ord_Non_EmpI = Svr_Ver_Ord_Non_Emp_def[THEN iffD2, rule_format]
+lemmas Svr_Ver_Ord_Non_EmpE[elim] = Svr_Ver_Ord_Non_Emp_def[THEN iffD1, elim_format, rule_format]
+         
+lemma reach_svr_ver_ord_non_emp [simp, dest]: "reach tapir s \<Longrightarrow> Svr_Ver_Ord_Non_Emp s k"
+proof(induction s rule: reach.induct)
+  case (reach_init s)
+  then show ?case
+  by (auto simp add: Svr_Ver_Ord_Non_Emp_def tapir_defs)
+next
+  case (reach_trans s e s')
+  then show ?case
+    by (induction e) (auto simp add: Svr_Ver_Ord_Non_Emp_def tapir_trans_defs)
+qed
+
+definition Svr_Ver_Ord_Cmt where
+  "Svr_Ver_Ord_Cmt s k \<longleftrightarrow> (\<forall>t \<in> set (svr_ver_order (svrs s k)).
+    (\<exists>ts rto v. svr_state (svrs s k) t = committed ts rto (Some v)))"
+                                                           
+lemmas Svr_Ver_Ord_CmtI = Svr_Ver_Ord_Cmt_def[THEN iffD2, rule_format]
+lemmas Svr_Ver_Ord_CmtE[elim] = Svr_Ver_Ord_Cmt_def[THEN iffD1, elim_format, rule_format]
+         
+lemma reach_svr_ver_ord_cmt [simp, dest]: "reach tapir s \<Longrightarrow> Svr_Ver_Ord_Cmt s k"
+proof(induction s rule: reach.induct)
+  case (reach_init s)
+  then show ?case
+  by (auto simp add: Svr_Ver_Ord_Cmt_def tapir_defs)
+next
+  case (reach_trans s e s')
+  then show ?case
+    by (induction e) (auto simp add: Svr_Ver_Ord_Cmt_def tapir_trans_defs)
+qed
+
+definition Read_Twr_Cmt where
+  "Read_Twr_Cmt s k \<longleftrightarrow> (\<forall>t t_wr ts wvo.
+    svr_state (svrs s k) t \<in> {read (Some t_wr),
+                              prepared ts (Some t_wr) wvo,
+                              committed ts (Some t_wr) wvo} \<longrightarrow> 
+    (\<exists>ts' rto' v. svr_state (svrs s k) t_wr = committed ts' rto' (Some v)))"
+                                                           
+lemmas Read_Twr_CmtI = Read_Twr_Cmt_def[THEN iffD2, rule_format]
+lemmas Read_Twr_CmtE[elim] = Read_Twr_Cmt_def[THEN iffD1, elim_format, rule_format]
+         
+lemma reach_read_t_wr_cmt [simp, dest]: "reach tapir s \<Longrightarrow> Read_Twr_Cmt s k"
+proof(induction s rule: reach.induct)
+  case (reach_init s)
+  then show ?case
+  by (auto simp add: Read_Twr_Cmt_def tapir_defs split: if_split_asm)
+next
+  case (reach_trans s e s')
+  then show ?case
+  proof (induction e)
+    case (Read_Resp x1 x2 x3)
+    then show ?case using Svr_Ver_Ord_Non_Emp_def[of s k] Svr_Ver_Ord_Cmt_def[of s k]
+      apply (simp add: Read_Twr_Cmt_def tapir_trans_defs)
+      by (smt last_in_set option.discI option.inject svr_state.distinct(5))
+  next
+    case (Prep x1 x2 x3 x4 x5a)
+    then show ?case
+      apply (simp add: Read_Twr_Cmt_def tapir_trans_defs)
+      by (smt Read_Twr_Cmt_def all_not_in_conv fun_upd_apply insert_iff occ_check_res
+          reach_trans.IH svr_state.distinct(9,11,13,15,17,19) svr_state.inject(2))
+  next
+    case (Commit x1 x2 x3 x4 x5a)
+    then show ?case
+      apply (auto simp add: Read_Twr_Cmt_def tapir_trans_defs)
+      by (metis svr_state.distinct(15))+
+  next
+    case (Abort x1 x2)
+    then show ?case
+      apply (simp add: Read_Twr_Cmt_def tapir_trans_defs)
+      by (metis svr_state.distinct(15) svr_state.distinct(19))
+  qed (auto simp add: Read_Twr_Cmt_def tapir_trans_defs)
+qed
 
 subsection \<open>Refinement Attempt\<close>
 
@@ -14,7 +107,7 @@ proof (intro simulate_ES_fun)
   fix gs0 :: "'v global_conf"
   assume p: "init tapir gs0"
   then show "init ET_SER.ET_ES (sim gs0)"
-    by (auto simp add: ET_SER.ET_ES_defs tapir_defs sim_defs kvs_init_def v_list_init_def 
+    by (auto simp add: ET_SER.ET_ES_defs tapir_defs sim_all_defs kvs_init_def v_list_init_def 
                        version_init_def)
 next
   fix gs a and gs' :: "'v global_conf"
@@ -56,22 +149,22 @@ next
         next 
           show \<open>fp_property F (kvs_of_s gs) u''\<close>
           proof -
-            have a: "\<And>k v. F k R = Some v \<Longrightarrow>
-              \<exists>t. svr_state (svrs gs k) (get_wtxn gs cl) = prepared ts (Some (v, t)) (F k W)"
-              using cmt
+            have a: "\<And>k t. r_map k = Some t \<Longrightarrow>
+              \<exists>ts rto v. svr_state (svrs gs k) t = committed ts rto (Some v)"
+              using cmt reach_s Read_Twr_Cmt_def[of gs]
               apply (auto simp add: cl_commit_def)
-              by (smt UnI1 UnI2 eq_fst_iff map_option_eq_Some option.distinct(1))
+              by (metis (no_types, lifting) Un_iff domI)
             show ?thesis using cmt
               apply (auto simp add: cl_commit_def fp_property_def view_snapshot_def)
-              subgoal for k v
-                using a[of k v] apply auto sorry.
-              (* Invariant: there is no timestamp inversion *)
-              (*apply (cases "svr_state (svrs gs k) (get_txn cl gs) = no_lock")
-              subgoal by (auto simp add: NoLockFpInv_def invariant_list_def)
-              subgoal by (smt (verit) RLockFpContentInv_def WLockFpContentInv_def
-                                      empty_iff insertCI insertE invariant_listE o_apply 
-                                      option.distinct(1) option.inject svr_vl_kvs_eq_lv) 
-              done*)
+              subgoal for k t_wr
+                using a[of k t_wr] apply auto
+            (* Invariant: there is no timestamp inversion *)
+            (*apply (cases "svr_state (svrs gs k) (get_txn cl gs) = no_lock")
+            subgoal by (auto simp add: NoLockFpInv_def invariant_list_def)
+            subgoal by (smt (verit) RLockFpContentInv_def WLockFpContentInv_def
+                                    empty_iff insertCI insertE invariant_listE o_apply 
+                                    option.distinct(1) option.inject svr_vl_kvs_eq_lv) 
+            done*) sorry sorry
           qed
         next 
           show \<open>kvs_of_s gs' = update_kv (Tn_cl sn cl) F u'' (kvs_of_s gs)\<close> using cmt (*I
@@ -90,38 +183,40 @@ next
   next
     case (Cl_Issue x1 x2 x3)
     then show ?case
-      apply (auto simp add: sim_defs tapir_trans_defs)
-      by (rule ext, auto simp add: sim_defs split: svr_state.split option.split)
+      apply (auto simp add: sim_def tapir_trans_defs)
+      by (rule ext, auto simp add: sim_all_defs split: svr_state.split option.split)
   next
     case (Cl_Read_Resp x1 x2 x3 x4)
     then show ?case
-      apply (auto simp add: sim_defs tapir_trans_defs)
-      by (rule ext, auto simp add: sim_defs split: svr_state.split option.split)
+      apply (auto simp add: sim_def tapir_trans_defs)
+      by (rule ext, auto simp add: sim_all_defs split: svr_state.split option.split)
   next
     case (Cl_Prep x1 x2 x3 x4)
     then show ?case
       apply (auto simp add: sim_def tapir_trans_defs)
-      by (rule ext, auto simp add: sim_defs split: svr_state.split option.split)
+      by (rule ext, auto simp add: sim_all_defs split: svr_state.split option.split)
   next
     case (Cl_Abort x)
     then show ?case
       apply (auto simp add: sim_def tapir_trans_defs)
-      by (rule ext, auto simp add: sim_defs split: svr_state.split option.split)+
+      by (rule ext, auto simp add: sim_all_defs split: svr_state.split option.split)+
   next
     case (Cl_ReadyC x1 x2)
     then show ?case
       apply (auto simp add: sim_def tapir_trans_defs)
-      apply (rule ext, auto simp add: sim_defs split: svr_state.split option.split) sorry
+       apply (rule ext, auto simp add: sim_all_defs split: svr_state.split option.split)
+      (* inv: new (uncommitted) write is not read by any transactions *)sorry
   next
     case (Cl_ReadyA x1 x2)
     then show ?case
       apply (auto simp add: sim_def tapir_trans_defs)
-      by (rule ext, auto simp add: sim_defs split: svr_state.split option.split)
+      by (rule ext, auto simp add: sim_all_defs split: svr_state.split option.split)
   next
     case (Read_Resp x1 x2 x3)
     then show ?case
+      using read_resp_abs_committed_reads_inv[of gs]
       apply (auto simp add: sim_defs tapir_trans_defs)
-      apply (rule ext, auto split: svr_state.split) sorry
+      by (rule ext, auto split: svr_state.split)
   next
     case (Prep x1 x2 x3 x4 x5)
     then show ?case sorry
